q3

A1/Q3.dfy
@@ -1,27 +1,3 @@
-/*
-MathUtils.reverseCantorPair = function(i)
-{
-    var pair = [];
-    var t = Math.floor((-1 + Math.sqrt(1 + 8 * i))/2);
-    var x = t * (t + 3) / 2 - i;
-    var y = i - t * (t + 1) / 2;
-    pair[0] = x;
-    pair[1] = y;
-    return pair;
-}
-
-*/
-/*
-How the sqrt function w==orks:
-Guess a number, in this case we use 'x'
-Check if x * x > target,z
-If it is, then find a new value that is the average of 'x' and the target number
-Check the new value recursively 
-Return 'x' if the product of itself is lower than the target value
-
-Check https://leetcode.com/problems/sqrtx/discuss/
-For iterative implementation of the sqrt function 
-*/
 function method findSum(sum : nat, next: nat, i : nat): (nat, nat)
 requires i >= 0;
 requires sum >= 0 && sum <= i;
@@ -29,6 +5,8 @@ requires next >= 0;
 decreases i - sum - next
 ensures sum <= i;
 {
+    //var x := i - sum;
+    //var y := next - x - 1;
     if (sum + next <= i) then findSum(sum + next, next + 1, i) else (i - sum, next - (i - sum) - 1)
 }
 
@@ -36,8 +14,6 @@ function method unpair (i: nat ): (nat, nat)
 requires i >= 0;
 { // TODO 
     var (x, y) := findSum(0, 0, i);
-    //var x := i - sum;
-    //var y := next - x - 1;
     var part := (x,y);
     part
 }
@@ -52,7 +28,24 @@ method catchTheSpy (a: nat , b: nat )
 {
     var i := 0;
     while a + i * b != pick (i)
+    invariant (a + b) >= findXYSum(i);
+    decreases ((a + b) - findXYSum(i)), findY(i); 
     { 
         i := i + 1; 
     }
 }
+
+function method findXYSum(i: nat): nat
+{
+    var (x, y) := unpair (i);
+    x + y
+}
+
+function method findY(i: nat): nat
+{
+    var (x, y) := unpair (i);
+    y
+}
+// a + i * b == x + i * y
+
+
